SkLean/Typing2.lean
@@ -1,75 +1,19 @@
 import SkLean.Ast2
 
-namespace valid_judgment_weak
+namespace valid_judgment
 
-lemma eval_preserves_judgment_hard : ∀ e e' t, valid_judgment_weak e t → is_eval_once e e' → valid_judgment_weak e' t := by
+lemma eval_preserves_judgment_hard : ∀ e e' t, valid_judgment e t → is_eval_once e e' → valid_judgment e' t := by
   intro e e' t h_t h_eval
-  cases h_t
-  case k n =>
+  induction h_t
+  cases h_eval
+  cases h_eval
+  cases h_eval
+  case call lhs rhs h_u h_t_lhs h_t_rhs ih₁ ih₂ =>
     cases h_eval
-  case s =>
-    cases h_eval
-  case m =>
-    cases h_eval
-  case call lhs rhs h_u h_t_lhs h_t_rhs  =>
-    match h₀ : h_eval with
-      | .k lhs' rhs' n =>
-        cases h_t_lhs
-      | .s x' y' z' n =>
-        cases h_t_lhs
-      | .left h_eval' =>
-        cases h_t_lhs
-      | .m e t n h_t =>
-        cases h_t_lhs
-
-lemma weakening : valid_judgment_weak e t → valid_judgment e t := by
-  intro h
-  cases h
-  case k =>
-    apply valid_judgment.k
-  case s =>
-    apply valid_judgment.s
-  case m =>
-    apply valid_judgment.m
-  case call lhs rhs h_u h_t_lhs h_t_rhs =>
-    apply valid_judgment.call
-    exact h_u
-    apply weakening at h_t_lhs
-    exact h_t_lhs
-    apply weakening at h_t_rhs
-    exact h_t_rhs
-
-lemma preserved : valid_judgment_weak e t → is_eval_once e e' → valid_judgment_weak e' t := by
-  intro h_t
-  sorry
-
-lemma imp_has_final_judgment_beta_eq : valid_judgment e t₁ → beta_eq t₁ t₂ → has_final_judgment e t₂ := by
-  intro h_t h_eq
-  apply has_final_judgment.hard
-  exact (beta_eq.symm h_eq)
-  cases h_t
-  case a.k =>
-    apply has_final_judgment.trivial
-    apply valid_judgment_weak.k
-  case a.s =>
-    apply has_final_judgment.trivial
-    apply valid_judgment_weak.s
-  case a.m =>
-    apply has_final_judgment.trivial
-    apply valid_judgment_weak.m
-  case a.call lhs rhs h_u h_t_lhs h_t_rhs =>
-    apply imp_has_final_judgment_call
-    exact h_u
-    exact h_t_lhs
-    exact h_t_rhs
-  sorry
-termination_by e
-
-end
-
-theorem preserved : valid_judgment e t → is_eval_once e e' → valid_judgment e' t := by
-  intro h_t h_eval
-  
-  sorry
+    cases h_t_lhs
+    cases h_t_lhs
+    cases h_t_lhs
+    cases h_t_lhs
+    cases h_t_lhs
 
 end valid_judgment
